Flapjack/Test/WordOperations.lean
@@ -58,6 +58,33 @@ def wordOperationSpillConfig : WordStackConfig :=
 
 example :
     wordToStackProgNat wordOperationSpillConfig
+        (.codeBufferWrite 0 1 : WordProg Nat) =
+      some (.seq (.stackLoad 29 13)
+        (.codeBufferWrite 29 6)) := by
+  simp [wordToStackProgNat, wordStackBufferWrite, wordStackLocation,
+    wordStackOffset, wordStackJoin, lookupNatInfo, wordOperationSpillConfig]
+
+example :
+    wordToStackProgNat wordOperationSpillConfig
+        (.dataBufferWrite 1 0 : WordProg Nat) =
+      some (.seq (.stackLoad 31 13)
+        (.dataBufferWrite 6 31)) := by
+  simp [wordToStackProgNat, wordStackBufferWrite, wordStackLocation,
+    wordStackOffset, wordStackJoin, lookupNatInfo, wordOperationSpillConfig]
+
+example :
+    wordToStackProgNat
+        { wordOperationSpillConfig with locations :=
+            [(0, .stack 3), (1, .stack 2)] }
+        (.codeBufferWrite 0 1 : WordProg Nat) =
+      some (.seq (.stackLoad 29 13)
+        (.seq (.stackLoad 31 12)
+          (.codeBufferWrite 29 31))) := by
+  simp [wordToStackProgNat, wordStackBufferWrite, wordStackLocation,
+    wordStackOffset, wordStackJoin, lookupNatInfo, wordOperationSpillConfig]
+
+example :
+    wordToStackProgNat wordOperationSpillConfig
         (.get 0 .heapLength : WordProg Nat) =
       some (.seq (.get 31 .heapLength) (.stackStore 31 13)) := by
   simp [wordToStackProgNat, wordStackGet, 
